It all builds!  Constructors are handled in a half-way decent fashion. Parameter-passing needs to be re-implemented in the same style as sub-constructor declarations.  Also, parameters need to allow for sub-classes being passed.  When parameter passing is done right, this will the same as allowing    Base *b = derivedptr; I don't know if it's legit but unadvised or flat-out illegal to pass a concrete derived to a function expecting a base.

holsrcs/class_infoScript.sml
@@ -11,33 +11,91 @@ open boolSimps
 open arithmeticTheory pred_setTheory integerTheory
 local
   open wordsTheory integer_wordTheory finite_mapTheory containerTheory
+       sortingTheory rich_listTheory
 in end
 
 (* C++ ancestor theories  *)
-open statesTheory
+open statesTheory aggregatesTheory
 
 val _ = new_theory "class_info";
 
-(* BAD_ASSUMPTION: for the moment, our hierarchies only allow one
-   ancestor class at most
-*)
+val cinfo_def = Define`
+  cinfo s cnm : class_info = FST (THE (s.classmap ' cnm))
+`;
+
+(* set of a state's fully defined class *)
+val defined_classes_def = Define`
+  defined_classes s = FDOM (deNONE s.classmap)
+`;
 
 (* c2 is an ancestor of c1 *)
 val ancestor_def = Define`
-  ancestor s c1 c2 = c1 IN FDOM (deNONE s.classmap) /\
-                     ((THE(s.classmap ' c1)).ancestors = SOME c2)
+  ancestor s c1 c2 =
+    c1 IN defined_classes s /\ ((cinfo s c1).ancestors = SOME c2)
 `;
+
 
 (* similarly, direct base classes, in order of declaration *)
 val get_direct_bases_def = Define`
   get_direct_bases s cnm : CPPname list =
-    [THE (THE (s.classmap ' cnm)).ancestors]
+    case (cinfo s cnm).ancestors of
+       NONE -> []
+    || SOME n -> [n]
 `
 
 val get_virtual_bases_def = Define`
   get_virtual_bases s cnm : CPPname list = []
 `;
 
+(* given a type, class-path pair, if the path is non-empty, then the
+   static type is Class of the last element in the path. *)
+val static_type_def = Define`
+  static_type (ty, pth) = if NULL pth then ty else Class (LAST pth)
+`;
+
+(* has any constructor, which seems to be the sense of what 8.5.1 p1 is
+   saying *)
+val has_user_constructor_def = Define`
+  has_user_constructor s cnm =
+    cnm IN defined_classes s /\
+    ?ci userdefined.
+       (s.classmap ' cnm = SOME (ci,userdefined)) /\
+       (DefaultConstructor IN userdefined \/ CopyConstructor IN userdefined)
+`;
+
+(* 8.5.1 p1 : aggregate types *)
+val is_aggregate_def = Define`
+  (is_aggregate s (Class cnm) =
+      ~has_user_constructor s cnm /\
+      (get_direct_bases s cnm = []) /\
+      (get_virtual_bases s cnm = []) /\
+      !fldname fldty prot.
+          MEM (FldDecl fldname fldty, F, prot) ((cinfo s cnm).fields) ==>
+          (prot = Public)) /\
+  (is_aggregate s _ = F)
+`;
+
+val strip_array_def = Define`
+  (strip_array (Array bt n) = strip_array bt) /\
+  (strip_array t = t)
+`;
+
+(* 9 p4  : POD types *)
+val (PODstruct_rules, PODstruct_ind, PODstruct_cases) = Hol_reln`
+  (!s cnm.
+     cnm IN defined_classes s /\
+     is_aggregate s (Class cnm) /\
+     DISJOINT {Destructor; CopyAssignment}
+              (SND (THE (s.classmap ' cnm))) /\
+     (!fldname fldty prot.
+         MEM (FldDecl fldname fldty, F, prot)
+             ((cinfo s cnm).fields) ==>
+         ~ref_type fldty /\
+         (!cnm'. (strip_array fldty = Class cnm') ==>
+                 PODstruct s cnm'))
+  ==>
+     PODstruct s cnm)
+`;
 
 (* Appending paths.  (Wasserab et al., section 3.4) *)
 val path_app_def = Define`
@@ -57,7 +115,7 @@ val _ = add_rule { block_style = (AroundEachPhrase, (PP.CONSISTENT, 0)),
 
 (* See the Subjobjs_R relation of Wasserab et al. *)
 val (rsubobjs_rules, rsubobjs_ind, rsubobjs_cases) = Hol_reln`
-  (!C s. C IN FDOM (deNONE s.classmap) ==> rsubobjs s (C, [C]))
+  (!C s. C IN defined_classes s ==> rsubobjs s (C, [C]))
 
     /\
 
@@ -70,7 +128,7 @@ val (rsubobjs_rules, rsubobjs_ind, rsubobjs_cases) = Hol_reln`
 val calc_rsubobjs = store_thm(
   "calc_rsubobjs",
   ``(C,Cs) IN rsubobjs s =
-       (Cs = [C]) /\ C IN FDOM (deNONE s.classmap) \/
+       (Cs = [C]) /\ C IN defined_classes s \/
        ?D Cs'. s |- C < D /\ (D,Cs') IN rsubobjs s /\
                  (Cs = C::Cs')``,
   SRW_TAC [][SPECIFICATION] THEN
@@ -150,10 +208,9 @@ val okfield_def = Define`
 val FieldDecls_def = Define`
   FieldDecls s C fnm =
      { (Cs, ty) | (C,Cs) IN subobjs s /\
-                  LAST Cs IN FDOM (deNONE s.classmap) /\
-                  ?cinfo centry staticp prot.
-                      (deNONE s.classmap ' (LAST Cs) = cinfo) /\
-                      MEM (centry,staticp,prot) cinfo.fields /\
+                  LAST Cs IN defined_classes s /\
+                  ?centry staticp prot.
+                      MEM (centry,staticp,prot) (cinfo s (LAST Cs)).fields /\
                       ~staticp /\
                       okfield centry /\
                       (fieldname centry = fnm) /\
@@ -185,126 +242,145 @@ val fieldty_via_def = Define`
 (* nsdmembers (non-static data-members) *)
 val nsdmembers_def = Define`
   nsdmembers s c =
-    case FLOOKUP (deNONE s.classmap) c of
-       NONE -> NONE
-    || SOME cinfo ->
-         SOME
-           (mapPartial
-              (\ci. case ci of
-                       (CFnDefn ret nm args bod, stat, prot) -> NONE
-                    || (FldDecl nm ty, stat, prot) -> if stat then NONE
-                                                      else SOME (nm,ty)
-                    || _ -> NONE)
-              cinfo.fields)
+    if c IN defined_classes s then
+      SOME
+        (mapPartial
+           (\ce. case ce of
+                    (CFnDefn ret nm args bod, stat, prot) -> NONE
+                 || (FldDecl nm ty, stat, prot) -> if stat then NONE
+                                                   else SOME (nm,ty)
+                 || _ -> NONE)
+           (cinfo s c).fields)
+    else NONE
 `
 
-(* p is the set of all the subobjs for a given class *)
-(* use of SET_TO_LIST means that one particular ordering of the set is taken
-   and used to determine the order in which the sub-objects appear *)
-val class_layout_def = Define`
-  class_layout (p : CPPname list set) = SET_TO_LIST p
-`
+val o_ABS_L = store_thm(
+  "o_ABS_L",
+  ``(\x. f x) o g = (\x. f (g x))``,
+  SRW_TAC [][combinTheory.o_DEF]);
 
-val class_layout_SING = store_thm(
-  "class_layout_SING",
-  ``class_layout {p} = [p]``,
-  SRW_TAC [][class_layout_def, containerTheory.SET_TO_LIST_THM, CHOICE_SING])
-val _ = export_rewrites ["class_layout_SING"]
+open utilsTheory
 
-(* This function is a little complicated because of inheritance.
-
-   Imagine a class hierarchy where B sits at the bottom, C is derived from
-   B, and D is derived from C.  Each of these classes has its own fields as
-   well: those things that appear between the braces when you write
-
-     class B { ... }
-
-   The sizeof function where this map is used expects to lookup a class name
-   and get back a list of things to look at further.  These things may be
-   normal fields, or more classes, which it will look up in turn.
-
-   The problem is that you don't want to look up D, learn that it
-   contains a B and C class, and then recursively look into the C,
-   learn that it contains a B etc.  You would then get multiple
-   unwarranted copies of ancestor classes.  Instead, when looking up a
-   genuine class, its hierarchy's classes are presented back as the
-   result of an intermediate calculation and the concatenation of the
-   non-static data members for those classes can be returned
-
+(* ASSUMPTION:
+     assume that virtual base classes must always appear last in the layout
+     of a class
 *)
+val get_class_constituents0_def = new_specification(
+  "get_class_constituents0_def",
+  ["get_class_constituents0"],
+  SIMP_RULE bool_ss [SKOLEM_THM]
+    (prove(``!s cnm. ?l.
+               PERM l (MAP (UNCURRY NSD) (THE (nsdmembers s cnm)) ++
+                       MAP DBase (get_direct_bases s cnm) ++
+                       MAP VirtualBase (get_virtual_bases s cnm)) /\
+               (mapPartial (\cc. case cc of NSD n ty -> SOME (n,ty)
+                                         || _ -> NONE) l =
+                THE (nsdmembers s cnm)) /\
+               (!i j vbnm. i < LENGTH l /\ j < LENGTH l /\ i < j /\
+                           (EL i l = VirtualBase vbnm) ==>
+                           ?vbnm'. EL j l = VirtualBase vbnm')``,
+            REPEAT GEN_TAC THEN
+            Q.HO_MATCH_ABBREV_TAC `?l. PERM l X /\ P l` THEN
+            Q.EXISTS_TAC `X` THEN SRW_TAC [][] THEN
+            Q.UNABBREV_ALL_TAC THEN
+            SRW_TAC [][mapPartial_MAP, o_ABS_L, mapPartial_K_NONE] THENL [
+              SRW_TAC [boolSimps.ETA_ss][pairTheory.UNCURRY,
+                                         mapPartial_SOME],
+              Q.HO_MATCH_ABBREV_TAC
+                `?vbnm'. EL j (l1 ++ l2 ++ l3) = VirtualBase vbnm'` THEN
+              Cases_on `i < LENGTH l1` THENL [
+                Q.PAT_ASSUM `EL i X = Y` MP_TAC THEN
+                FULL_SIMP_TAC (srw_ss() ++ ARITH_ss)
+                              [rich_listTheory.EL_APPEND1] THEN
+                Q.UNABBREV_TAC `l1` THEN
+                FULL_SIMP_TAC (srw_ss()) [rich_listTheory.EL_MAP] THEN
+                Cases_on `EL i (THE (nsdmembers s cnm))` THEN
+                SRW_TAC [][],
+                ALL_TAC
+              ] THEN
+              `l1 ++ l2 ++ l3 = l1 ++ (l2 ++ l3)` by SRW_TAC [][] THEN
+              FULL_SIMP_TAC (bool_ss ++ ARITH_ss)
+                            [rich_listTheory.EL_APPEND2] THEN
+              Q.ABBREV_TAC `i' = i - LENGTH l1` THEN
+              Cases_on `i' < LENGTH l2` THENL [
+                Q.PAT_ASSUM `EL i' X = Y` MP_TAC THEN
+                FULL_SIMP_TAC (srw_ss()) [rich_listTheory.EL_APPEND1,
+                                          Abbr`l2`, rich_listTheory.EL_MAP],
+                ALL_TAC
+              ] THEN
+              `i' < j - LENGTH l1` by SRW_TAC [ARITH_ss][Abbr`i'`] THEN
+              FULL_SIMP_TAC (srw_ss() ++ ARITH_ss)
+                            [rich_listTheory.EL_APPEND2, Abbr`l3`] THEN
+              Q_TAC SUFF_TAC `j - (LENGTH l1 + LENGTH l2) <
+                              LENGTH
+                                (MAP VirtualBase (get_virtual_bases s cnm))`
+                    THEN1 SRW_TAC [][rich_listTheory.EL_MAP] THEN
+              Q.UNABBREV_ALL_TAC THEN
+              FULL_SIMP_TAC (srw_ss() ++ ARITH_ss)[]
+            ])))
 
-val class_szmap_def = Define`
-   class_szmap s =
-      FUN_FMAP
-         (\c. let subs = class_layout { so | (c,so) IN subobjs s }
-                          (* get "subobjects", which includes the most
-                             derived class name *)
-              in
-                      (* the end of the path in the subobj is the name of the
-                         class, get its nsdmembers, map SND to strip out
-                         the field names, and flatten the result *)
-                 FLAT (MAP (\p. MAP SND (THE (nsdmembers s (LAST p)))) subs))
-         (FDOM (deNONE s.classmap))
+val get_class_constituents_def = Define`
+  get_class_constituents s mdp cnm =
+     FILTER (\cc. case cc of VirtualBase _ -> mdp || x -> T)
+            (get_class_constituents0 s cnm)
+`;
+
+val sizeofmap_def = Define`
+  sizeofmap s mdp =
+     FUN_FMAP (get_class_constituents s mdp) (FDOM s.classmap)
 `
 
-(* SANITY *)
-val FDOM_class_szmap = store_thm(
-  "FDOM_class_szmap",
-  ``FDOM (class_szmap s) = FDOM (deNONE s.classmap)``,
-  SRW_TAC [][class_szmap_def, finite_mapTheory.FUN_FMAP_DEF])
-val _ = export_rewrites ["FDOM_class_szmap"]
 
-
-val genoffset_def = Define`
-  (genoffset [] acc szf alnf e = NONE) /\
-  (genoffset (h::t) (acc:num) szf alnf e =
-    let acc' = roundup (alnf h) acc
-    in
-      if h = e then SOME acc'
-      else genoffset t (acc' + szf h) szf alnf e)
-`
-val _ = export_rewrites ["genoffset_def"]
-
-(* given derived class name C, state s, and path to base sub-object p, return
-   the offset of the latter within an object of type C *)
-val subobj_offset_def = Define`
-  subobj_offset s C p =
-    let tyfm = class_szmap s
-    in
-      genoffset
-        (class_layout { so | (C,so) IN subobjs s})
-        0
-        (\pth. if nsdmembers s (LAST pth) = SOME [] then 0
-               else
-                 @sz. sizeof tyfm (Class (LAST pth)) sz)
-        (\pth. if nsdmembers s (LAST pth) = SOME [] then 0
-               else @a. align tyfm (Class (LAST pth)) a)
-        p
-`
-
-
-val nsds_bases_def = Define`
-  nsds_bases s cnm =
-    let layout = class_layout { so | (cnm, so) IN subobjs s } in
-    let info p =
-      let off = THE (subobj_offset s cnm p)
+(* calculates the offset of a virtual base within particular class, assuming
+   it is most-derived *)
+val virtual_offset_def = Define`
+  virtual_offset s C1 C2 =
+      let ccs = get_class_constituents s T C1 in
+      let i = THE (LFINDi ((=) (VirtualBase C2)) ccs)
       in
-          if p = [cnm] then
-            let nsds = THE (nsdmembers s cnm)
-            in
-              MAP (\ (fld,ty).
-                   (SOME fld, ty,
-                    THE (genoffset nsds off
-                              (\ (nm,ty). @sz. sizeof (class_szmap s) ty sz)
-                              (\ (nm,ty). @a. align (class_szmap s) ty a)
-                              (fld,ty))))
-                  nsds
-          else [(NONE, Class (LAST p), off)]
-    in
-      FLAT (MAP info layout)
+        @off. offset (sizeofmap s) ccs i off
 `
 
+val base_offset_def = Define`
+  base_offset s C1 C2 =
+      let ccs = get_class_constituents0 s C1 in
+      let i = THE (LFINDi ((=) (DBase C2)) ccs)
+      in
+        @off. offset (sizeofmap s) ccs i off
+`;
 
+val constituent_offsets_def = Define`
+  constituent_offsets s mdp cnm =
+    let ccs = get_class_constituents s mdp cnm in
+    let nccs = NUMBER 0 ccs
+    in
+        MAP (\(n,c). (c, @off. offset (sizeofmap s) ccs n off)) nccs
+`;
+
+val init_order_offsets_def = Define`
+  init_order_offsets s mdp cnm =
+    let virts : CPPname list = if mdp then get_virtual_bases s cnm else [] in
+    let dbases : CPPname list  = get_direct_bases s cnm in
+    let nsds = THE (nsdmembers s cnm) in
+    let all = MAP VirtualBase virts ++ MAP DBase dbases ++
+              MAP (UNCURRY NSD) nsds in
+    let all_layout_order = get_class_constituents s mdp cnm in
+    let alli = MAP (\cc. (cc, THE (LFINDi ((=) cc) all_layout_order))) all
+    in
+        MAP (\(cc,i). (cc, @off. offset (sizeofmap s) all_layout_order i off))
+            alli
+`
+
+(* given derived class name C, state s, and path to (not necessarily
+   immediate) base sub-class p, return the offset of the latter
+   within an object of type C *)
+val subobj_offset_def = Define`
+  (subobj_offset s (C1, [C2]) = if C1 = C2 then 0
+                                else virtual_offset s C1 C2) /\
+  (subobj_offset s (C1, (C2::C3::t)) =
+               (* C1 must equal C2 *)
+               base_offset s C1 C3 + subobj_offset s (C3, (C3::t)))
+`
 
 (* BAD ASSUMPTION: no classes are abstract *)
 (* type-checking requires a variety of pieces of information, which we derive
@@ -317,13 +393,6 @@ val expr_type_comps_def = Define`
                              (s.classmap ' c = SOME v) };
        var_types := s.typemap ;
        abs_classes := {} |>
-`;
-
-(* sizeof calculations expect to find a map from class name to a list
-   of types (the class's (non-static) fields.  This function calculates
-   that map from a classmap *)
-val sizeofmap_def = Define`
-  sizeofmap s = class_szmap s
 `;
 
 val MEM_splits = prove(
@@ -339,12 +408,7 @@ val hasfld_imp_lfi = store_thm(
   "hasfld_imp_lfi",
   ``s |- C has least fld -: ftype via p' /\ object_type ftype ==>
     ?i. lookup_field_info (THE (nsdmembers s (LAST p'))) fld (i,ftype)``,
-  SRW_TAC [][fieldty_via_def, FieldDecls_def, nsdmembers_def,
-             finite_mapTheory.FLOOKUP_DEF] THEN
-  Q.SPEC_THEN `deNONE s.classmap ' (LAST p')`
-              STRIP_ASSUME_TAC
-              statementsTheory.class_info_literal_nchotomy THEN
-  FULL_SIMP_TAC (srw_ss()) [] THEN
+  SRW_TAC [][fieldty_via_def, FieldDecls_def, nsdmembers_def] THEN
   Cases_on `centry` THEN
   FULL_SIMP_TAC (srw_ss()) [fieldtype_def, typesTheory.object_type_def,
                             okfield_def] THEN
