holsrcs/aggregatesScript.sml
@@ -1,0 +1,371 @@
+(* Calculating sizes for types, and offsets for objects within classes *)
+
+(* Michael Norrish *)
+
+(* pro-forma *)
+open HolKernel boolLib Parse bossLib BasicProvers
+open boolSimps
+
+(* Standard HOL ancestory theories *)
+open arithmeticTheory pred_setTheory integerTheory
+local
+  open wordsTheory integer_wordTheory finite_mapTheory containerTheory
+       sortingTheory rich_listTheory dividesTheory
+in end
+
+(* C++ ancestor theories  *)
+open memoryTheory typesTheory
+
+val _ = new_theory "aggregates";
+
+
+val _ = Hol_datatype`
+  class_constituent = NSD of string => CPP_Type
+                    | DBase of CPPname
+                    | VirtualBase of CPPname
+`;
+
+val cc_case_MONO = store_thm(
+  "cc_case_MONO",
+  ``(!s ty. nsf s ty ==> nsf' s ty) /\ (!n. bf n ==> bf' n) /\
+    (!n. vf n ==> vf' n) ==>
+    (class_constituent_case nsf bf vf v ==>
+     class_constituent_case nsf' bf' vf' v)``,
+  Cases_on `v` THEN SRW_TAC [][]);
+val _ = export_mono "cc_case_MONO"
+
+val cc_type_def = Define`
+  (cc_type (NSD nm ty) = ty) /\
+  (cc_type (VirtualBase cnm) = Class cnm) /\
+  (cc_type (DBase cnm) = Class cnm)
+`;
+val _ = export_rewrites ["cc_type_def"]
+
+val nsdp_def = Define`
+  (nsdp (NSD nm ty) = T) /\
+  (nsdp _ = F)
+`;
+val _ = export_rewrites ["nsdp_def"]
+
+val empty_base_size_def = new_specification(
+  "empty_base_size_def",
+  ["empty_base_size"],
+  SIMP_RULE bool_ss [SKOLEM_THM]
+  (prove(``?n. 0n <= n``, SRW_TAC [][])))
+
+val empty_base_align_def = new_specification(
+  "empty_base_align_def",
+  ["empty_base_align"],
+  (prove(``?n. 0n <= n /\ n <= empty_base_size``,
+         Q.EXISTS_TAC `0` THEN SRW_TAC [][])))
+
+
+val (empty_class_rules, empty_class_ind, empty_class_cases) = Hol_reln`
+  (!cnm.
+       EVERY (\cc. case cc of
+                      DBase n -> empty_class s F n
+                   || VirtualBase n -> empty_class s F n
+                   || NSD nm ty -> F)
+             (s mdp ' cnm)
+   ==>
+       empty_class s mdp cnm)
+`;
+
+(* SANITY *)
+val nil_empty_class = store_thm(
+  "nil_empty_class",
+  ``(s mdp ' cnm = []) ==> empty_class s mdp cnm``,
+  SRW_TAC [][Once empty_class_cases]);
+
+val lcml_def = Define`
+  (lcml [] = 1) /\
+  (lcml (h::t) = lcm h (lcml t))
+`;
+
+val (align_rules, align_ind, align_cases) = Hol_reln`
+  (!smap mdp. align smap mdp BChar 1) /\  (* same as Char *)
+
+  (!smap mdp. align smap mdp Bool bool_align) /\
+
+  (!smap mdp ty. align smap mdp (Signed ty) (bit_align ty)) /\
+
+  (!smap mdp ty. align smap mdp (Unsigned ty) (bit_align ty)) /\
+
+  (!smap mdp ty. align smap mdp (Ptr ty) (ptr_align ty)) /\
+
+  (* BAD_ASSUMPTION *)
+  (!smap mdp c ty. align smap mdp (MPtr c ty) (ptr_align ty)) /\
+
+  (!smap mdp ty n a. align smap T ty a ==> align smap mdp (Array ty n) a) /\
+
+  (!smap mdp cnm aligns.
+      cnm IN FDOM (smap mdp) /\ ~empty_class smap mdp cnm /\
+      listRel (cc_align smap) (smap mdp ' cnm) aligns
+         ==>
+      align smap mdp (Class cnm) (lcml aligns))
+
+   /\
+
+   (!smap mdp cnm.
+      cnm IN FDOM (smap mdp) /\ empty_class smap mdp cnm ==>
+      align smap mdp (Class cnm) empty_class_align)
+
+   /\
+
+
+   (!smap nm ty a.
+     align smap T ty a
+   ==>
+     cc_align smap (NSD nm ty) a)
+
+   /\
+
+
+   (!smap cnm.
+     empty_class smap F cnm
+   ==>
+     cc_align smap (DBase cnm) empty_base_align)
+
+   /\
+
+   (!smap cnm.
+     empty_class smap F cnm
+   ==>
+     cc_align smap (VirtualBase cnm) empty_base_align)
+
+   /\
+
+   (!smap cnm a.
+     ~empty_class smap F cnm /\ align smap F (Class cnm) a
+   ==>
+     cc_align smap (DBase cnm) a)
+
+   /\
+
+   (!smap cnm a.
+     ~empty_class smap F cnm /\ align smap F (Class cnm) a
+   ==>
+     cc_align smap (VirtualBase cnm) a)
+`;
+
+(* SANITY : alignment relation is deterministic *)
+val align_det = store_thm(
+  "align_det",
+  ``(!smap mdp ty a. align smap mdp ty a ==>
+                     !b. align smap mdp ty b ==> (a = b)) /\
+    (!smap cc a. cc_align smap cc a ==> !b. cc_align smap cc b ==> (a = b))``,
+  HO_MATCH_MP_TAC align_ind THEN REPEAT CONJ_TAC THEN
+  REPEAT GEN_TAC THEN
+  ((Q.MATCH_ABBREV_TAC `align U X Y Z ==> P` THEN
+    Q.UNABBREV_ALL_TAC THEN
+    ONCE_REWRITE_TAC [align_cases]) ORELSE
+   (STRIP_TAC THEN ONCE_REWRITE_TAC [align_cases])) THEN
+  SRW_TAC [][] THEN
+  Q_TAC SUFF_TAC `aligns = aligns'` THEN1 SRW_TAC [][] THEN
+  NTAC 2 (POP_ASSUM MP_TAC) THEN
+  Q_TAC SUFF_TAC
+        `!ccs als. listRel (cc_align smap) ccs als ==>
+                   !als'. listRel (\cc a. !b. cc_align smap cc b ==> (a = b))
+                                  ccs
+                                  als' ==>
+                          (als = als')` THEN1 METIS_TAC [] THEN
+  HO_MATCH_MP_TAC listTheory.listRel_ind THEN SRW_TAC [][] THEN
+  FULL_SIMP_TAC (srw_ss()) [listTheory.listRel_CONS]);
+
+(* SANITY: cc_alignment on NSDs is the same as align *)
+val ccalign_NSD = store_thm(
+  "ccalign_NSD",
+  ``cc_align s (NSD nm ty) a = align s T ty a``,
+  CONV_TAC (LAND_CONV (ONCE_REWRITE_CONV [align_cases])) THEN
+  SRW_TAC [][]);
+val _ = export_rewrites ["ccalign_NSD"]
+
+(* SANITY *)
+val align_int = store_thm(
+  "align_int",
+  ``(align smap mdp (Signed Int) a = (a = int_align)) /\
+    (align smap mdp (Unsigned Int) a = (a = int_align))``,
+  ONCE_REWRITE_TAC [align_cases] THEN SRW_TAC [][])
+val _ = export_rewrites ["align_int"]
+
+val align_char = store_thm(
+  "align_char",
+  ``(align smap mdp (Signed Char) a = (a = 1)) /\
+    (align smap mdp (Unsigned Char) a = (a = 1)) /\
+    (align smap mdp BChar a = (a = 1))``,
+  ONCE_REWRITE_TAC [align_cases] THEN SRW_TAC [][])
+val _ = export_rewrites ["align_char"]
+
+(* ----------------------------------------------------------------------
+    type sizes and field offsets within classes
+   ---------------------------------------------------------------------- *)
+
+val roundup_def = Define`
+  roundup base n = if n MOD base = 0 then n else (n DIV base + 1) * base
+`;
+
+
+
+(* sizeof :
+     bool -> (bool -> CPPname |-> class_constituent list) -> CPP_Type ->
+     num -> bool
+
+   First:  bool indicates whether or not the type is a most-derived class
+   Second: bool -> finite-map returns the constituents of a class, the
+           boolean is true if the class is "most-derived".
+   Third:  type to find size
+   Fourth: the size
+*)
+val (sizeof_rules, sizeof_ind, sizeof_cases) = Hol_reln`
+
+  (!s mdp. sizeof mdp s BChar 1) /\
+
+  (!s mdp. sizeof mdp s Bool bool_size) /\
+
+  (!s b mdp. sizeof mdp s (Signed b) (bit_size b)) /\
+
+  (!s b mdp. sizeof mdp s (Unsigned b) (bit_size b)) /\
+
+  (!s t mdp. sizeof mdp s (Ptr t) (ptr_size t)) /\
+
+  (!s c t mdp. sizeof mdp s (MPtr c t) (ptr_size t)) /\ (* BAD_ASSUMPTION *)
+
+  (!s m n t mdp.
+     sizeof mdp s t m
+  ==>
+     sizeof mdp s (Array t n) (m * n))
+
+  /\
+
+  (!s c mdp cclist a lastoff lastsz.
+        c IN FDOM (s mdp) /\
+        (cclist = s mdp ' c) /\ ~empty_class s mdp c /\
+        align s mdp (Class c) a /\
+        offset s cclist (LENGTH cclist - 1) lastoff /\
+        ccsizeof s (EL (LENGTH cclist - 1) cclist) lastsz
+      ==>
+        sizeof mdp s (Class c) (roundup a (lastoff + lastsz)))
+
+  /\
+
+  (!s c mdp.
+    c IN FDOM (s mdp) /\ empty_class s mdp c
+  ==>
+    sizeof mdp s (Class c) empty_class_size)
+
+  /\
+
+
+  (!s c f.
+    c IN FDOM (s F) /\ empty_class s F c /\ ((f = VirtualBase) \/ (f = DBase))
+  ==>
+    ccsizeof s (f c) empty_base_size)
+
+  /\
+
+  (!f s c sz.
+    c IN FDOM (s F) /\ ~empty_class s F c /\
+    sizeof F s (Class c) sz /\ ((f = VirtualBase) \/ (f = DBase))
+  ==>
+    ccsizeof s (f c) sz)
+
+  /\
+
+  (!s nm ty sz.
+    sizeof T s ty sz
+  ==>
+    ccsizeof s (NSD nm ty) sz)
+
+  /\
+
+  (!s cclist.  offset s cclist 0 0) /\
+  (!s cclist n a offn sizen.
+        offset s cclist n offn /\
+        ccsizeof s (EL n cclist) sizen /\
+        cc_align s (EL (SUC n) cclist) a
+      ==>
+        offset s cclist (SUC n) (roundup a (offn + sizen)))
+`;
+
+
+(* SANITY: sizeof and offset are deterministic *)
+val det_lemma = prove(
+  ``(!mdp s ty n. sizeof mdp s ty n ==> !m. sizeof mdp s ty m ==> (n = m)) /\
+    (!s cc n. ccsizeof s cc n ==> !m. ccsizeof s cc m ==> (n = m)) /\
+    (!s tylist n off1.
+              offset s tylist n off1 ==>
+              !off2. offset s tylist n off2 ==> (off1 = off2))``,
+  HO_MATCH_MP_TAC sizeof_ind THEN REPEAT CONJ_TAC THEN
+  REPEAT GEN_TAC THEN
+  TRY (ONCE_REWRITE_TAC [sizeof_cases] THEN SRW_TAC [][] THEN NO_TAC)
+  THENL [
+    (* array *)
+    STRIP_TAC THEN ONCE_REWRITE_TAC [sizeof_cases] THEN SRW_TAC [][] THEN
+    METIS_TAC [],
+    (* non-empty class size *)
+    STRIP_TAC THEN ONCE_REWRITE_TAC [sizeof_cases] THEN SRW_TAC [][] THEN
+    FULL_SIMP_TAC (srw_ss()) [] THEN METIS_TAC [align_det],
+    (* empty class size *)
+    STRIP_TAC THEN ONCE_REWRITE_TAC [sizeof_cases] THEN SRW_TAC [][] THEN
+    RES_TAC,
+    (* cc non-empty base *)
+    SRW_TAC [][] THEN POP_ASSUM MP_TAC THEN
+    ONCE_REWRITE_TAC [sizeof_cases] THEN SRW_TAC [][] THEN RES_TAC,
+    (* cc NSD *)
+    STRIP_TAC THEN ONCE_REWRITE_TAC [sizeof_cases] THEN SRW_TAC [][] THEN
+    RES_TAC,
+    (* offset SUC *)
+    STRIP_TAC THEN ONCE_REWRITE_TAC [sizeof_cases] THEN SRW_TAC [][] THEN
+    METIS_TAC [align_det, listTheory.EL]
+  ])
+val sizeof_det = save_thm("sizeof_det", CONJUNCT1 det_lemma)
+val ccsizeof_det = save_thm("offset_det", CONJUNCT1 (CONJUNCT2 det_lemma))
+val offset_det = save_thm("offset_det", CONJUNCT2 (CONJUNCT2 det_lemma))
+
+(* SANITY: only object types have sizes *)
+val only_objects_have_sizes = store_thm(
+  "only_objects_have_sizes",
+  ``!mdp s ty n. sizeof mdp s ty n ==> object_type ty``,
+  ONCE_REWRITE_TAC [sizeof_cases] THEN SRW_TAC [][object_type_def] THEN
+  SRW_TAC [][]);
+
+(* SANITY: for example, functions don't have sizes *)
+val functions_have_no_size = store_thm(
+  "functions_have_no_size",
+  ``~sizeof mdp s (Function retty argtys) n``,
+  STRIP_TAC THEN IMP_RES_TAC only_objects_have_sizes THEN
+  FULL_SIMP_TAC (srw_ss()) [object_type_def])
+
+(* SANITY *)
+val ccsizeof_NSD = store_thm(
+  "ccsizeof_NSD",
+  ``ccsizeof smap (NSD nm ty) sz = sizeof T smap ty sz``,
+  CONV_TAC (LAND_CONV (ONCE_REWRITE_CONV [sizeof_cases])) THEN
+  SRW_TAC [boolSimps.DNF_ss][]);
+val _ = export_rewrites ["ccsizeof_NSD"]
+
+(* SANITY *)
+val sizeof_char = store_thm(
+  "sizeof_char",
+  ``(sizeof mdp smap (Signed Char) sz = (sz = 1)) /\
+    (sizeof mdp smap (Unsigned Char) sz = (sz = 1)) /\
+    (sizeof mdp smap BChar sz = (sz = 1))``,
+  ONCE_REWRITE_TAC [sizeof_cases] THEN SRW_TAC [][])
+val _ = export_rewrites ["sizeof_char"]
+
+(* SANITY *)
+val sizeof_int = store_thm(
+  "sizeof_int",
+  ``(sizeof mdp smap (Signed Int) sz = (sz = int_size)) /\
+    (sizeof mdp smap (Unsigned Int) sz = (sz = int_size))``,
+  ONCE_REWRITE_TAC [sizeof_cases] THEN SRW_TAC [][]);
+val _ = export_rewrites ["sizeof_int"]
+
+val offset_0 = store_thm(
+  "offset_0",
+  ``offset smap els 0 off = (off = 0)``,
+  ONCE_REWRITE_TAC [sizeof_cases] THEN SRW_TAC [][]);
+val _ = export_rewrites ["offset_0"]
+
+
+val _ = export_theory();
